plugin/Extract.v
@@ -1,2 +1,2 @@
 From Malfunction.Plugin Require Import Loader.
-From Malfunction.Plugin Require Export PrimInt63 PrimFloats PrimArray CoqMsgFFI.
+From Malfunction.Plugin Require Export PrimInt63 PrimFloat PrimArray CoqMsgFFI.
